src/Parsers/Reflective/LogicalRelations.v
@@ -155,10 +155,14 @@ Proof.
   rewrite <- IHxs, H; reflexivity.
 Qed.
 
+Lemma bool_rect_nodep_const {P x b}
+  : BoolFacts.Bool.bool_rect_nodep P x x b = x.
+Proof. destruct b; reflexivity. Qed.
+
 Create HintDb partial_unfold_hints discriminated.
 
 Hint Rewrite <- @interp_Term_syntactify_list @interp_Term_syntactify_nat @List.map_rev : partial_unfold_hints.
-Hint Rewrite @nth'_nth List.map_nth List.map_map List.map_length List.map_id @combine_map_r @combine_map_l @first_index_default_map Bool.orb_true_r Bool.orb_true_l Bool.andb_true_l Bool.andb_true_r Bool.orb_false_r Bool.orb_false_l Bool.andb_false_l Bool.andb_false_r BoolFacts.andbr_andb BoolFacts.orbr_orb : partial_unfold_hints.
+Hint Rewrite @nth'_nth List.map_nth List.map_map List.map_length List.map_id @combine_map_r @combine_map_l @first_index_default_map Bool.orb_true_r Bool.orb_true_l Bool.andb_true_l Bool.andb_true_r Bool.orb_false_r Bool.orb_false_l Bool.andb_false_l Bool.andb_false_r BoolFacts.andbr_andb BoolFacts.orbr_orb @bool_rect_nodep_const : partial_unfold_hints.
 Hint Resolve map_ext_in fold_left_app (@constantOf_correct cbool) @first_index_default_first_index_partial : partial_unfold_hints.
 
 Local Ltac meaning_tac_helper' :=
@@ -266,6 +270,8 @@ Local Ltac simpler_meaning :=
          | [ H : ?x = _ |- context[?x] ] => rewrite H
          | [ H : context[match constantOf ?x with _ => _ end] |- _ ]
            => destruct (constantOf x) eqn:?
+         | [ H : match ?T with cbool => _ | _ => _ end _ = Some _ |- _ ]
+           => is_var T; destruct T
          end.
 
 Lemma list_rect_nodep_meaning_correct {A : SimpleTypeCode} {P} f f' n n'
