src/Parsers/Reflective/ParserSemantics.v
@@ -10,18 +10,19 @@ Require Import Fiat.Common.Wf Fiat.Common.Wf2.
 Set Implicit Arguments.
 
 Definition step_option_rec
+           {T}
            (is_valid_nonterminal : list nat -> nat -> bool)
            (len0 valid_len0 : nat)
            (parse_nt : forall len0' valid_len : nat,
                Wf.prod_relation lt lt (len0', valid_len) (len0, valid_len0) ->
-               list nat -> nat -> forall len : nat, len <= len0' -> nat -> bool)
+               list nat -> nat -> forall len : nat, len <= len0' -> nat -> T)
            (G_length : nat)
            (up_to_G_length : list nat)
            (valids : list nat) (offset len : nat)
            (nt : nat)
-  : option (nat -> nat -> nat -> bool).
+  : option (nat -> nat -> nat -> T).
 Proof.
-  refine (sumbool_rect (fun _ => option (nat -> nat -> nat -> bool))
+  refine (sumbool_rect (fun _ => option (nat -> nat -> nat -> T))
                        (fun pf =>
                           Some
                             (fun offset' len0_minus_len'
@@ -34,7 +35,7 @@ Proof.
                         => _)
                        (Compare_dec.lt_dec len len0)).
   refine (sumbool_rect
-            (fun _ => option (nat -> nat -> nat -> bool))
+            (fun _ => option (nat -> nat -> nat -> T))
             (fun is_valid
              => _)
             (fun _ => None)
@@ -48,35 +49,37 @@ Proof.
   apply (proj1 (proj1 (Bool.andb_true_iff _ _) is_valid)).
 Defined.
 
-Definition interp_has_parse_term
+Definition interp_has_parse_term'
+           {T}
+           (interp_Term : forall {T}, Term interp_TypeCode T -> interp_TypeCode T)
            (is_valid_nonterminal : list nat -> nat -> bool)
            (strlen : nat)
            (char_at_matches_interp : nat -> Reflective.RCharExpr Ascii.ascii -> bool)
            (split_string_for_production : nat * (nat * nat) -> nat -> nat -> list nat)
-           (t : has_parse_term interp_TypeCode) : bool
+           (t : has_parse_term interp_TypeCode T) : interp_TypeCode T
   := match t with
-     | RFix2 G_length up_to_G_length f valid_len valids nt_idx
+     | RFix2 G_length up_to_G_length f default valid_len valids nt_idx
        => Wf2.Fix2
             (Wf.well_founded_prod_relation Wf_nat.lt_wf Wf_nat.lt_wf)
             (fun aa' : nat * nat =>
-               list nat -> nat -> forall a1 : nat, a1 <= fst aa' -> nat -> bool)
+               list nat -> nat -> forall a1 : nat, a1 <= fst aa' -> nat -> interp_TypeCode T)
             (fun (len0 valid_len0 : nat)
                  (parse_nt : forall len0' valid_len : nat,
                      Wf.prod_relation lt lt (len0', valid_len) (len0, valid_len0) ->
-                     list nat -> nat -> forall len : nat, len <= len0' -> nat -> bool)
+                     list nat -> nat -> forall len : nat, len <= len0' -> nat -> interp_TypeCode T)
                  (valids : list nat) (offset len : nat)
                  (pf : len <= len0)
                  (nt : nat)
              => option_rect
-                  (fun _ : option (interp_TypeCode (cnat --> cnat --> cnat --> cbool)) => bool)
+                  (fun _ : option (interp_TypeCode (cnat --> cnat --> cnat --> T)) => interp_TypeCode T)
                   (fun parse_nt
                    => interp_Term
                         f
                         (fun n : interp_TypeCode cnat => char_at_matches_interp n (*str*))
                         (fun n : interp_TypeCode (cnat * (cnat * cnat)) => split_string_for_production n (*str*))
                         len0 valid_len parse_nt valids offset len nt)
-                  false
-                  (@step_option_rec is_valid_nonterminal len0 valid_len0 parse_nt G_length up_to_G_length valids offset len nt))
+                  (interp_Term default)
+                  (@step_option_rec (interp_TypeCode T) is_valid_nonterminal len0 valid_len0 parse_nt G_length up_to_G_length valids offset len nt))
             strlen
             valid_len
             valids
@@ -85,3 +88,6 @@ Definition interp_has_parse_term
             (le_n _)
             nt_idx
      end.
+
+Definition interp_has_parse_term {T}
+  := Eval cbv [interp_has_parse_term'] in @interp_has_parse_term' T (@interp_Term).
